Translation validate that toLinear input is linearizable

compiler/lvcc.ml
@@ -25,6 +25,8 @@ let implode l =
     | c :: l -> Bytes.set res i c; imp (i + 1) l in
   imp 0 l;;
 
+exception NotLinearizableException
+
 let main () =
   (* Give identifiert i, n the lowest indexes, do force
      heuristic to pick them. *)
@@ -93,6 +95,9 @@ let main () =
 	else
 	  ili
       in
+      let _ = if not (IsLinearizable.isLinearizableStmt s_fromILF) then
+		raise (Compiler_error "The statement is not linearizable.\nThis can happen if the input program was not fully scheduled.\nI.e. there are let-bindings that do not correspond to instructions.\nIf -s was uses, it can also mean that some instructions used non-register arguments.")
+	      else () in
       let linear = ToLinear.coq_ILItoLinear (Camlcoq.P.of_int !num_registers) s_fromILF in
       let _ = PrintMach.destination := Some machname in
       let asm =
