theories/Infra/Indexwise.v
@@ -3,17 +3,34 @@ Require Export Infra.Option EqDec AutoIndTac Get.
 
 Set Implicit Arguments.
 
+Definition indexwise_P {A} (P:A -> Prop) LA :=
+  forall n a, get LA n a -> P a.
+
+Definition indexwise_P_dec {A} {P:A->Prop} LA
+           (Rdec:(forall n a, get LA n a -> Computable (P a)))
+      : Computable (indexwise_P P LA).
+unfold Computable. revert LA Rdec. fix 1. intros LA Rdec.
+destruct LA; try now left; isabsurd.
+intros. destruct (Rdec 0 a).
+- eauto using get.
+- destruct (indexwise_P_dec LA).
+  + intros. eauto using get.
+  + clear indexwise_P_dec. left; hnf; intros; inv H; eauto.
+  + right; intro HH. eapply n; hnf; intros; eapply HH; eauto using get.
+- right; intro. eapply n; hnf; intros. eapply H; eauto using get.
+Defined.
+
 Definition indexwise_R {A} {B} (R:A->B->Prop) LA LB :=
 forall n a b, get LA n a -> get LB n b -> R a b.
 
-Definition indexwise_R2_dec {A} {B} {R:A->B->Prop} LA LB (Rdec:(forall n a b, get LA n a -> get LB n b -> Computable (R a b)))
+Definition indexwise_R_dec {A} {B} {R:A->B->Prop} LA LB (Rdec:(forall n a b, get LA n a -> get LB n b -> Computable (R a b)))
       : Computable (indexwise_R R LA LB).
 unfold Computable. revert LA LB Rdec. fix 2. intros LA LB Rdec.
 destruct LA, LB; try now left; isabsurd.
 intros. destruct (Rdec 0 a b).
 - eauto using get.
 - eauto using get.
-- destruct (indexwise_R2_dec LA LB).
+- destruct (indexwise_R_dec LA LB).
   + intros. eauto using get.
   + left. hnf; intros. destruct n; inv H; inv H0; eauto.
   + right; intro HH. eapply n; hnf; intros; eapply HH; eauto using get.
